verif/btrees.v
@@ -285,8 +285,9 @@ Fixpoint findRecordIndex' {X:Type} (le:listentry X) (key:key) (i:index): index :
     end
   end.
 
-Definition findRecordIndex {X:Type} (le:listentry X) (key:key) : index :=
-  findRecordIndex' le key (ip O).
+Definition findRecordIndex {X:Type} (n:node X) (key:key) : index :=
+    match n with btnode ptr0 le b F L x =>
+                 findRecordIndex' le key (ip O) end.
 
 (* updates a child in a listentry *)
 Fixpoint update_le_nth_child {X:Type} (i:nat) (le:listentry X) (n:node X) : listentry X :=
