verif/btrees_spec.v
@@ -157,16 +157,15 @@ Definition findChildIndex_spec : ident * funspec :=
 
 Definition findRecordIndex_spec : ident * funspec :=
   DECLARE _findRecordIndex
-  WITH le:listentry val, key:key, p:val
-  PRE[ _entries OF tptr tentry, _key OF tuint, _length OF tint ]
-  PROP(p<>nullval)
-  LOCAL(temp _length (Vint (Int.repr (Z.of_nat (numKeys_le le))));
-        temp _key (Vint (Int.repr key)))
-  SEP(le_iter_sepcon le; valid_pointer p)
+  WITH n:node val, key:key, p:val
+  PRE[ _node OF tptr tbtnode, _key OF tuint ]
+  PROP(LeafNode n)
+  LOCAL(temp _node p; temp _key (Vint (Int.repr key)))
+  SEP(btnode_rep n p)
   POST[ tint ]
   PROP()
-  LOCAL(temp ret_temp (rep_index(findRecordIndex le key)))
-  SEP(le_iter_sepcon le; valid_pointer p).
+  LOCAL(temp ret_temp (rep_index(findRecordIndex n key)))
+  SEP(btnode_rep n p).
 
 (**
     GPROG
