verif/verif_findindex.v
@@ -79,7 +79,226 @@ Proof.
     entailer!.
     assert((numKeys (btnode val ptr0 (cons val (keychild val k n0) le') false First Last p)) = S (numKeys_le le')). simpl. auto.
     rewrite H1.
-    forward_if.
+    unfold abbreviate in POSTCONDITION.
+
+(*   check_Delta; check_POSTCONDITION; *)
+(*  repeat apply -> semax_seq_skip; *)
+(*  repeat (apply seq_assoc1; try apply -> semax_seq_skip). *)
+(*   apply semax_if_seq. *)
+(* match goal with *)
+(* | |- semax ?Delta (PROPx ?P (LOCALx ?Q (SEPx ?R))) (Sifthenelse ?e ?c1 ?c2) _ => *)
+(*    let HRE := fresh "H" in let v := fresh "v" in *)
+(*     evar (v: val); *)
+(*     do_compute_expr Delta P Q R e v HRE; *)
+(*     simpl in v; *)
+(*     apply (semax_ifthenelse_PQR' _ v); *)
+(*     [ reflexivity  *)
+(*       | ..(* | entailer | assumption *)
+(*      | clear HRE; subst v; apply semax_extract_PROP; intro HRE; *)
+(*        do_repr_inj HRE; *)
+(*        repeat (apply semax_extract_PROP; intro); *)
+(*        try rewrite Int.signed_repr in HRE by rep_omega; *)
+(*        abbreviate_semax *)
+(*      | clear HRE; subst v; apply semax_extract_PROP; intro HRE; *)
+(*        do_repr_inj HRE; *)
+(*        repeat (apply semax_extract_PROP; intro); *)
+(*        try rewrite Int.signed_repr in HRE by rep_omega; *)
+(*        abbreviate_semax*) *)
+(*      ] *)
+(* (* | |- semax ?Delta (PROPx ?P (LOCALx ?Q (SEPx ?R))) (Ssequence (Sifthenelse ?e ?c1 ?c2) _) _ => *) *)
+(* (*     tryif (unify (orb (quickflow c1 nofallthrough) (quickflow c2 nofallthrough)) true) *) *)
+(* (*     then (apply semax_if_seq; forward_if'_new) *) *)
+(* (*     else fail 100 "Because your if-statement is followed by another statement, you need to do 'forward_if Post', where Post is a postcondition of type (environ->mpred) or of type Prop" *) *)
+(* (* | |- semax _ (@exp _ _ _ _) _ _ => *) *)
+(* (*       fail 100 "First use Intros ... to take care of the EXistentially quantified variables in the precondition" *) *)
+(* (* | |- semax _ _ (Sswitch _ _) _ => *) *)
+(* (*   forward_switch' *) *)
+(* (* | |- semax _ _ (Ssequence (Sifthenelse _ _ _) _) _ =>  *) *)
+(* (*      fail 100 "forward_if failed for some unknown reason, perhaps your precondition is not in canonical form" *) *)
+(* (* | |- semax _ _ (Ssequence (Sswitch _ _) _) _ =>  *) *)
+(* (*      fail 100 "Because your switch statement is followed by another statement, you need to do 'forward_if Post', where Post is a postcondition of type (environ->mpred) or of type Prop" *) *)
+(* end. *)
+(* Ltac try_conjuncts_solver ::= *)
+(*   lazymatch goal with H:_ |- ?A => *)
+(*          no_evars A; *)
+(*          clear H; try immediate; auto; prove_it_now; fail *)
+(*   end. *)
+
+(* clear. simpl tc_expr. go_lower. clear. *)
+
+
+(*  intros; *)
+(*  try match goal with POSTCONDITION := @abbreviate ret_assert _ |- _ => *)
+(*         clear POSTCONDITION *)
+(*       end; *)
+(*  try match goal with MORE_COMMANDS := @abbreviate statement _ |- _ => *)
+(*         clear MORE_COMMANDS *)
+(*       end; *)
+(*  match goal with *)
+(*  | |- local _ && ?P |-- _ => go_lower; try simple apply empTrue *)
+(*  | |- ?P |-- _ => *)
+(*     match type of P with *)
+(*     | ?T => unify T mpred; pull_out_props *)
+(*     end *)
+(*  | |- _ => fail "The entailer tactic works only on entailments  _ |-- _ " *)
+(*  end. *)
+(*  saturate_local. *)
+(*  ent_iter. *)
+(*  simple apply prop_right. simpl. clear. *)
+(*  rewrite ?isptr_force_ptr by auto. *)
+(*  let H := fresh in eapply my_auto_lem. *)
+(*  intro H. *)
+(*  instantiate (1:=True) in H. *)
+(*  rewrite ?intsigned_intrepr_bytesigned. *)
+(* Locate rep_omega. *)
+
+(*  repeat match goal with *)
+(*             |  x:= _ : Z |- _ => subst x *)
+(*             |  x:= _ : nat |- _ => subst x *)
+(*             |  x:= _ |- _ => clearbody x *)
+(*             end; *)
+(*   try autorewrite with rep_omega in *. *)
+(*   unfold repable_signed in *. *)
+(*   pose_Zlength_nonneg. *)
+(*   pose_lemmas Byte.unsigned byte_unsigned' Byte.unsigned_range. *)
+(*   pose_lemmas Byte.signed byte_signed' Byte.signed_range. *)
+(*   pose_lemmas Int.unsigned int_unsigned' Int.unsigned_range. *)
+(*   Locate pose_lemmas. *)
+(*   match goal with *)
+(*     |- context [Int.signed ?A] => *)
+(*     match type of (Int.signed_range A) with ?T => *)
+(*                                             pose proof (Int.signed_range A) *)
+(*     end *)
+(*   end. *)
+
+  (* match goal with *)
+  (*                 |- context [Int.signed ?A] => *)
+  (*                 change (Int.signed A) with (int_signed' A) in * *)
+  (* end. *)
+  
+  (* forward_if calls rep_omega *)
+  (* which calls rep_omega_setup *)
+  (* which calls pose_lemmas Int.signed int_signed' Int.signed_range *)
+  (* which calls pose_lemma Int.signed int_signed' A Int.signed_range *)
+  (* which calls   match goal with *)
+  (*                 |- context [Int.signed ?A] => *)
+  (*                 change (Int.signed A) with (int_signed' A) in * *)
+  (*               end. *)
+  (* And this 'change' tactic takes forever. *)
+  
+
+(*   match goal with *)
+(*     |- context [Int.signed ?A] => *)
+(*                                               change (Int.signed A) with (int_signed' A) in * *)
+(*   end. *)
+
+  
+(*   match goal with *)
+(*     |- context [Int.signed ?A] => *)
+(*     match type of (Int.signed_range A) with ?T => *)
+(*                              lazymatch goal with *)
+(*                              | H:  T |- _ => idtac *)
+(*                              | H:  T /\ _ |- _ => idtac *)
+(*                              | |- _ => pose proof (Int.signed_range A) *)
+(*                              end;  change (Int.signed A) with (int_signed' A) in * *)
+(*     end *)
+(*   end. *)
+  
+(*   match goal with *)
+(*     |- context [Int.signed ?A] => pose_lemma Int.signed int_signed' A Int.signed_range *)
+(*   end. *)
+
+
+
+  
+  
+(*  repeat *)
+(*   match goal with *)
+(*   | |- context [Int.signed ?A] => pose_lemma Int.signed int_signed' A Int.signed_range *)
+(*   | H: context [Int.signed ?A] |- _ => pose_lemma Int.signed int_signed' A Int.signed_range *)
+(* (*  | H:= context [Int.signed ?A] |- _ => pose_lemma F int_signed' A L *) *)
+(*  end; *)
+(*   unfold int_signed' in *. *)
+
+
+(*   pose_lemmas Int.signed int_signed' Int.signed_range. *)
+(*   pose_lemmas Int64.unsigned int64_unsigned' Int64.unsigned_range; *)
+(*   pose_lemmas Int64.signed int64_unsigned' Int64.signed_range; *)
+(*   pose_lemmas Ptrofs.unsigned ptrofs_unsigned' Ptrofs.unsigned_range; *)
+(*   pose_standard_const_equations. *)
+
+
+(* rep_omega_setup. *)
+
+
+
+
+(*    rep_omega2. *)
+
+
+
+(*  rep_omega (* Omega0 *). *)
+(*  first [ splittable; fail 1 *)
+(*         | computable *)
+(*         | apply Coq.Init.Logic.I *)
+(*         | reflexivity *)
+(*         | rewrite ?intsigned_intrepr_bytesigned; rep_omega (* Omega0 *) *)
+(*         | prove_signed_range *)
+(*         | repeat match goal with H: ?A |- _ => has_evar A; clear H end; *)
+(*           auto with prove_it_now field_compatible; *)
+(*           autorewrite with norm entailer_rewrite; normalize; *)
+(*           first [eapply field_compatible_nullval; eassumption *)
+(*                  | eapply field_compatible_nullval1; eassumption *)
+(*                  | eapply field_compatible_nullval2; eassumption *)
+(*                  ] *)
+(*          ]. *)
+
+
+
+
+(*  prove_it_now. *)
+(*  first [instantiate (1:=True) in H;  prove_it_now *)
+(*        | splittable; *)
+(*          eapply try_conjuncts_lem; *)
+(*             [let H1 := fresh in intro H1; my_auto_iter H1 *)
+(*             |let H1 := fresh in intro H1; my_auto_iter H1 *)
+(*             | apply H ] *)
+(*        | apply H *)
+(*        ]. *)
+
+
+
+
+(*  my_auto_iter H. *)
+(*  [intro H; my_auto_iter H | ]. *)
+(*  try all_True; *)
+(*  (eapply my_auto_lem; [intro; my_auto_reiter | ]); *)
+(*  normalize. *)
+
+
+
+
+(*  unfold numKeys_le. my_auto. *)
+(*  first [ contradiction *)
+(*         | simple apply prop_right; my_auto *)
+(*         | match goal with |- ?Q |-- !! _ && ?Q' => constr_eq  Q Q'; *)
+(*                       simple apply prop_and_same_derives'; my_auto *)
+(*           end *)
+(*         | simple apply andp_right; *)
+(*             [apply prop_right; my_auto  *)
+(*             | cancel; rewrite <- ?sepcon_assoc; autorewrite with norm ] *)
+(*         | normalize; cancel; rewrite <- ?sepcon_assoc *)
+(*         ]. *)
+
+
+
+
+(* entailer!. *)
+
+(*     forward_if. *)
+
+
+    
     (* why is this forward_if so long? *)
 
 Admitted.
@@ -88,5 +307,54 @@ Admitted.
 Lemma body_findRecordIndex: semax_body Vprog Gprog f_findRecordIndex findRecordIndex_spec.
 Proof.
   start_function.
+  forward.                      (* i=0 *)
+  destruct n as [ptr0 le isLeaf First Last x].
+  pose (n:= btnode val ptr0 le isLeaf First Last x). fold n.
+  forward_if (PROP ( ) LOCAL (temp _i (Vint (Int.repr 0)); temp _node p; temp _key (Vint (Int.repr key))) SEP (btnode_rep n p)).
+  - apply denote_tc_test_eq_split.
+    admit.
+    entailer!.
+  - forward.                    (* skip *)
+    entailer!.
+  - assert_PROP(False). unfold btnode_rep. entailer!.
+    admit.                      (* offset_val 20 p = nullval should be a contradiction? *)
+    contradiction.
+  - rewrite unfold_btnode_rep. unfold n. Intros. subst x.
+    forward.                    (* t'5=node->numKeys *)
+    gather_SEP 0 1 2 3 4 5 6 7.
+    replace_SEP 0 (btnode_rep n p).
+    entailer!.
+    { forward_if(PROP ( ) LOCAL (temp _t'5 (Vint (Int.repr (Z.of_nat (numKeys (btnode val ptr0 le isLeaf First Last p))))); temp _i (Vint (Int.repr 0)); temp _node p; temp _key (Vint (Int.repr key))) SEP (btnode_rep n p)).
+      - forward.                (* skip *)
+        entailer!.
+      - admit.
+        (* contradiction in H0 *)
+      - rewrite unfold_btnode_rep. unfold n. Intros.
+        forward.                (* t'4=node->numKeys *)
+        forward_if.
+        + forward.              (* return *)
+          entailer!.
+          assert(le= nil val). admit. (* true from H0 *)
+          rewrite H12. simpl. auto.
+        + forward.              (* skip *)
+          forward.              (* i=0 *)
+          gather_SEP 0 1 2 3 4 5 6 7.
+          replace_SEP 0 (btnode_rep n p).
+          entailer!. deadvars!.
+{ forward_loop (EX i:Z, (PROP (i<= Z.of_nat (numKeys_le le))
+     LOCAL (temp _i (Vint (Int.repr i)); temp _node p; temp _key (Vint (Int.repr key)))
+     SEP (btnode_rep n p)))
+               break:(EX i:Z, (PROP (i= Z.of_nat(numKeys_le le))
+     LOCAL (temp _i (Vint (Int.repr i)); temp _node p; temp _key (Vint (Int.repr key)))
+     SEP (btnode_rep n p))).
+  - Exists 0. entailer!.
+  - Intros i. rewrite unfold_btnode_rep. unfold n. Intros.
+    forward.                    (* t'3=node->numKeys *)
+    (* forward_if. => this one is stuck too*)
+    admit.
+  - Intros i. rewrite unfold_btnode_rep. unfold n. Intros.
+    forward.                    (* t'1=node->numKeys *)
+    forward.                    (* return *)
+    entailer!.
+    admit.                      (* loop invariant isn't strong enough *)
 Admitted.
-
